I_1(q_r,q_{\theta},\tau)&=C_1\left[1-\exp(-v_1q_r\tau)\right]
+C_2\left[q_r\exp\left(-\frac{q_r}{\lambda}\right)\right]\left[\tau\exp\left(-\frac{\tau}{\tau_2}\right)\right]\cos(v_2q_r\tau)\cos(q_{\theta}+\phi) \\
I_2(q_r,q_{\theta},\tau)&=C_1\left[1-\exp\left(-\frac{\tau}{\tau_1}\right)\right]
+C_2\left[q_r\exp\left(-\frac{q_r}{\lambda}\right)\right]\left[\tau\exp\left(-\frac{\tau}{\tau_2}\right)\right]\cos(v_2q_r\tau)\cos(q_{\theta}+\phi) \\
I_3(q_r,q_{\theta},\tau)&=C_1\left[1-\exp(-v_1q_r\tau)\right]
+C_2\left[\exp\left(-\frac{q_r}{\lambda}\right)\right]\left[\exp\left(-\frac{\tau}{\tau_2}\right)\right]\sin(v_2q_r\tau)\cos(q_{\theta}+\phi) \\
I_4(q_r,q_{\theta},\tau)&=C_1\left[1-\exp\left(-\frac{\tau}{\tau_1}\right)\right]
+C_2\left[\exp\left(-\frac{q_r}{\lambda}\right)\right]\left[\exp\left(-\frac{\tau}{\tau_2}\right)\right]\sin(v_2q_r\tau)\cos(q_{\theta}+\phi)
